src/Assembly/PipelineExample.v
@@ -2,32 +2,48 @@
 Require Import Pseudo Qhasm AlmostQhasm Conversion Language.
 Require Import PseudoConversion AlmostConversion StringConversion.
 
-Module P64 := Pseudo PseudoUnary64.
-Module C64 := PseudoConversion PseudoUnary64.
+Extraction Language Ocaml.
+Require Import ExtrOcamlString ExtrOcamlBasic.
+Require Import Coq.Strings.String.
 
-Import C64.P.
+Module Progs.
+  Module P64 := Pseudo PseudoUnary64.
+  Module C64 := PseudoConversion PseudoUnary64.
 
-Definition prog0: Pseudo 1 1.
-  refine (PBin _ Wplus
-      (PVar 1 (exist _ 0 _))
-      (PConst _ (natToWord _ 1)));
-    abstract intuition.
-Defined.
+  Import C64.P.
 
-Definition prog1: option AlmostQhasm.Program :=
-  C64.Conv.convertProgram prog0.
+  Definition prog0: Pseudo 1 1.
+    refine (PBin _ Wplus
+        (PVar 1 (exist _ 0 _))
+        (PConst _ (natToWord _ 1)));
+        abstract intuition.
+  Defined.
 
-Definition prog2: option Qhasm.Program :=
-  match prog1 with
-  | Some p => AlmostConversion.convertProgram p
-  | None => None
-  end.
+  Definition prog1: option AlmostQhasm.Program :=
+    C64.Conv.convertProgram prog0.
 
-Definition prog3: option string :=
-  match prog2 with
-  | Some p => StringConversion.convertProgram p
-  | None => None
-  end.
+  Definition prog2: option Qhasm.Program :=
+    match prog1 with
+    | Some p => AlmostConversion.convertProgram p
+    | None => None
+    end.
 
-Eval compute in prog3.
+  Definition prog3: string :=
+    match prog2 with
+    | Some p =>
+        match (StringConversion.convertProgram p) with
+        | Some s => s
+        | None => EmptyString
+        end
+    | None => EmptyString
+    end.
 
+  Definition result: string.
+    let res := eval vm_compute in prog3 in exact res.
+  Defined.
+
+  Open Scope string_scope.
+  Print result.
+End Progs.
+
+(* Extraction "Progs.ml" Progs. *)
